Remove candle

basis/basis_ffi.c
@@ -465,8 +465,7 @@ int main (int local_argc, char **local_argv) {
 
   /* Set up the signal handler for SIGINTs when running the REPL. */
   for (int i = 0; i < local_argc; i++) {
-      if (strcmp(local_argv[i], "--repl") == 0 ||
-          strcmp(local_argv[i], "--candle") == 0) {
+      if (strcmp(local_argv[i], "--repl") == 0) {
         signal(SIGINT, do_sigint);
         break;
       }
