candle/standard/ml_kernel/runtime_checkLib.sig
@@ -1,7 +1,0 @@
-signature runtime_checkLib = sig
-
-  include Abbrev
-
-  val check : term quotation list -> thm -> thm
-
-end
