compiler/bootstrap/compilation/x64/64/candle_records.ml
@@ -1,1 +1,0 @@
-../../../../../candle/prover/candle_records.ml
