compiler/repl/repl_decs_allowedScript.sml
@@ -4,7 +4,7 @@
 *)
 open preamble
 open semanticsPropsTheory evaluateTheory semanticPrimitivesTheory
-open candle_prover_invTheory
+open ast_extrasTheory
 
 val _ = Parse.hide "types"
 
@@ -14,8 +14,55 @@ val _ = patternMatchesLib.ENABLE_PMATCH_CASES();
 
 (* definition *)
 
+Definition safe_exp_def:
+  safe_exp = every_exp $ λx.
+               case x of
+                | _ => T
+End
+
+Theorem safe_exp_simps[simp] =
+   [“safe_exp (Raise e)”,
+    “safe_exp (Handle e pes)”,
+    “safe_exp (Lit lit)”,
+    “safe_exp (Con opt xs)”,
+    “safe_exp (Var n)”,
+    “safe_exp (Fun n x)”,
+    “safe_exp (App op xs)”,
+    “safe_exp (Log lop x y)”,
+    “safe_exp (If x y z)”,
+    “safe_exp (Mat e pes)”,
+    “safe_exp (Let opt x y)”,
+    “safe_exp (Letrec f x)”,
+    “safe_exp (Tannot e t)”,
+    “safe_exp (Lannot e l)”]
+  |> map (SIMP_CONV (srw_ss()) [safe_exp_def])
+  |> map (SIMP_RULE (srw_ss()) [GSYM safe_exp_def, SF ETA_ss])
+  |> LIST_CONJ;
+
+Definition safe_dec_def:
+  safe_dec = every_dec $ λd.
+               case d of
+                 Dlet locs pat x => safe_exp x
+               | Dletrec locs funs => EVERY safe_exp (MAP (SND o SND) funs)
+               | _ => T
+End
+
+Theorem safe_dec_simps[simp] =
+  [“safe_dec (Dlet l p x)”,
+   “safe_dec (Dletrec l f)”,
+   “safe_dec (Dtype l tds)”,
+   “safe_dec (Dtabbrev l ns n t)”,
+   “safe_dec (Dexn l n ts)”,
+   “safe_dec (Dmod mn ds)”,
+   “safe_dec (Dlocal ds1 ds2)”,
+   “safe_dec (Denv n)”]
+  |> map (SIMP_CONV (srw_ss()) [safe_dec_def])
+  |> map (SIMP_RULE (srw_ss()) [GSYM safe_dec_def, SF ETA_ss])
+  |> LIST_CONJ;
+
+
 Definition decs_allowed_def:
-  decs_allowed (decs:ast$dec list) = EVERY candle_prover_inv$safe_dec decs
+  decs_allowed (decs:ast$dec list) = EVERY safe_dec decs
 End
 
 (* pmatch lemmas *)
@@ -23,10 +70,6 @@ End
 Triviality safe_exp_pmatch_lemma:
   safe_exp =
      every_exp $ λx. case x of
-                     | Con opt xs => (dtcase opt of
-                                      | SOME id => let n = id_to_n id in n ∉ kernel_ctors
-                                      | NONE => T)
-                     | App op xs' => op ≠ FFI kernel_ffi
                      | _ => T
 Proof
   CONV_TAC(ONCE_DEPTH_CONV patternMatchesLib.PMATCH_ELIM_CONV)
@@ -38,8 +81,6 @@ Proof
 QED
 
 Theorem safe_exp_pmatch = safe_exp_pmatch_lemma
-  |> SIMP_RULE std_ss [candle_kernel_valsTheory.kernel_ctors_def,
-                       candle_kernel_valsTheory.kernel_ffi_def,
-                       IN_UNION,IN_INSERT,NOT_IN_EMPTY,GSYM CONJ_ASSOC]
+  |> SIMP_RULE std_ss [IN_UNION,IN_INSERT,NOT_IN_EMPTY,GSYM CONJ_ASSOC]
 
 val _ = export_theory();
