candle/syntax-lib/README.md
@@ -1,4 +1,0 @@
-Auxiliary definitions used for manipulating (deeply embedded) HOL syntax.
-
-[holSyntaxLibScript.sml](holSyntaxLibScript.sml):
-Definitions for manipulating (deeply embedded) HOL syntax.
